Launchbury/ArityAnalysisFix.thy
@@ -173,5 +173,95 @@ lemma Afix_cong[fundef_cong]:
       \<Longrightarrow> ArityAnalysis.Afix aexp1 heap1 = ArityAnalysis.Afix aexp2 heap2"
    unfolding ArityAnalysis.Afix_def by (metis Abinds_cong)
 
+
+context EdomArityAnalysis
+begin
+
+lemma Afix_edom: "edom (Afix \<Gamma> \<cdot> ae) \<subseteq> fv \<Gamma> \<union> edom ae"
+  unfolding Afix_eq
+  by (rule fix_ind[where P = "\<lambda> ae' . edom ae' \<subseteq> fv \<Gamma> \<union> edom ae"] )
+     (auto dest: set_mp[OF edom_AnalBinds])
+
+lemma ABinds_lookup_fresh:
+  "atom v \<sharp> \<Gamma> \<Longrightarrow> (ABinds \<Gamma>\<cdot>ae) v = \<bottom>"
+by (induct \<Gamma> rule: ABinds.induct) (auto simp add: fresh_Cons fresh_Pair fup_Aexp_lookup_fresh fresh_delete)
+
+lemma Afix_lookup_fresh:
+  assumes "atom v \<sharp> \<Gamma>"
+  shows "(Afix \<Gamma>\<cdot>ae) v = ae v"
+  apply (rule below_antisym)
+  apply (subst Afix_eq)
+  apply (rule fix_ind[where  P = "\<lambda> ae'. ae' v \<sqsubseteq> ae v"])
+  apply (auto simp add: ABinds_lookup_fresh[OF assms] fun_belowD[OF Afix_above_arg])
+  done
+
+lemma Afix_comp2join_fresh:
+  "atom ` (domA \<Delta>) \<sharp>* \<Gamma> \<Longrightarrow> ABinds \<Delta>\<cdot>(Afix \<Gamma>\<cdot>ae) = ABinds \<Delta>\<cdot>ae"
+proof (induct \<Delta> rule: ABinds.induct)
+  case 1 show ?case by (simp add: Afix_above_arg del: fun_meet_simp)
+next
+  case (2 v e \<Delta>)
+  from 2(2)
+  have "atom v \<sharp> \<Gamma>" and  "atom ` domA (delete v \<Delta>) \<sharp>* \<Gamma>"
+    by (auto simp add: fresh_star_def)
+  from 2(1)[OF this(2)]
+  show ?case by (simp del: fun_meet_simp add: Afix_lookup_fresh[OF `atom v \<sharp> \<Gamma>`])
+qed
+
+lemma Afix_append_fresh:
+  assumes "atom ` domA \<Delta> \<sharp>* \<Gamma>"
+  shows "Afix (\<Delta> @ \<Gamma>)\<cdot>ae = Afix \<Gamma>\<cdot>(Afix \<Delta>\<cdot>ae)"
+proof (rule below_antisym)
+  show *: "Afix (\<Delta> @ \<Gamma>)\<cdot>ae \<sqsubseteq> Afix \<Gamma>\<cdot>(Afix \<Delta>\<cdot>ae)"
+  apply (rule Afix_least_below)
+  apply (simp add: Abinds_append_disjoint[OF fresh_distinct[OF assms]] Afix_comp2join_fresh[OF assms])
+  apply (rule below_trans[OF join_mono[OF Abinds_Afix_below Abinds_Afix_below]])
+  apply (simp_all add: Afix_above_arg  below_trans[OF Afix_above_arg Afix_above_arg])
+  done
+next
+  show "Afix \<Gamma>\<cdot>(Afix \<Delta>\<cdot>ae) \<sqsubseteq> Afix (\<Delta> @ \<Gamma>)\<cdot>ae"
+  proof (rule Afix_least_below)
+    show "ABinds \<Gamma>\<cdot>(Afix (\<Delta> @ \<Gamma>)\<cdot>ae) \<sqsubseteq> Afix (\<Delta> @ \<Gamma>)\<cdot>ae"
+      apply (rule below_trans[OF _ Abinds_Afix_below])
+      apply (subst Abinds_append_disjoint[OF fresh_distinct[OF assms]])
+      apply simp
+      done
+    have "ABinds \<Delta>\<cdot>(Afix (\<Delta> @ \<Gamma>)\<cdot>ae) \<sqsubseteq> Afix (\<Delta> @ \<Gamma>)\<cdot>ae"
+      apply (rule below_trans[OF _ Abinds_Afix_below])
+      apply (subst Abinds_append_disjoint[OF fresh_distinct[OF assms]])
+      apply simp
+      done
+    thus "Afix \<Delta>\<cdot>ae \<sqsubseteq> Afix (\<Delta> @ \<Gamma>)\<cdot>ae"
+      apply (rule Afix_least_below)
+      apply (rule Afix_above_arg)
+      done
+  qed
+qed
+
+
+lemma Afix_e_to_heap:
+   "Afix (delete x \<Gamma>)\<cdot>(fup\<cdot>(Aexp e)\<cdot>n \<squnion> ae) \<sqsubseteq> Afix ((x, e) # delete x \<Gamma>)\<cdot>(esing x\<cdot>n \<squnion> ae)"
+    apply (simp add: Afix_eq)
+    apply (rule fix_least_below, simp)
+    apply (intro join_below)
+    apply (subst fix_eq, simp)
+    apply (subst fix_eq, simp)
+
+    apply (rule below_trans[OF _ join_above2])
+    apply (rule below_trans[OF _ join_above2])
+    apply (rule below_trans[OF _ join_above2])
+    apply (rule monofun_cfun_arg)
+    apply (subst fix_eq, simp)
+      
+    apply (subst fix_eq, simp) back apply (simp add: below_trans[OF _ join_above2])
+    done
+
+lemma Afix_e_to_heap':
+   "Afix (delete x \<Gamma>)\<cdot>(Aexp e\<cdot>n) \<sqsubseteq> Afix ((x, e) # delete x \<Gamma>)\<cdot>(esing x\<cdot>(up\<cdot>n))"
+using Afix_e_to_heap[where ae = \<bottom> and n = "up\<cdot>n"] by simp
+
+end
+
+
 end
 
