Launchbury/ArityAnalysisSpec.thy
@@ -2,22 +2,6 @@ theory ArityAnalysisSpec
 imports ArityAnalysisAbinds
 begin
 
-locale EdomArityAnalysis = ArityAnalysis + 
-  assumes Aexp_edom: "edom (Aexp e\<cdot>a) \<subseteq> fv e"
-begin
-
-  lemma fup_Aexp_edom: "edom (fup\<cdot>(Aexp e)\<cdot>a) \<subseteq> fv e"
-    by (cases a) (auto dest:set_mp[OF Aexp_edom])
-  
-  lemma Aexp_fresh_bot[simp]: assumes "atom v \<sharp> e" shows "(Aexp e\<cdot>a) v = \<bottom>"
-  proof-
-    from assms have "v \<notin> fv e" by (metis fv_not_fresh)
-    with Aexp_edom have "v \<notin> edom (Aexp e\<cdot>a)" by auto
-    thus ?thesis unfolding edom_def by simp
-  qed
-
-end
-
 locale SubstArityAnalysis = EdomArityAnalysis + 
   assumes Aexp_subst_restr: "x \<notin> S \<Longrightarrow> y \<notin> S \<Longrightarrow> (Aexp e[x::=y] \<cdot> a) f|` S = (Aexp e\<cdot>a) f|` S"
 
@@ -26,27 +10,15 @@ locale CorrectArityAnalysis = SubstArityAnalysis +
   assumes Aexp_App: "Aexp e \<cdot>(inc\<cdot>n) \<squnion> esing x \<cdot> (up\<cdot>0) \<sqsubseteq>  Aexp (App e x) \<cdot> n"
   assumes Aexp_Lam: "env_delete y (Aexp e \<cdot>(pred\<cdot>n)) \<sqsubseteq> Aexp (Lam [y]. e) \<cdot> n"
 
-locale CorrectArityAnalysisAheap = CorrectArityAnalysis + 
-  fixes Aheap :: "heap \<Rightarrow> exp \<Rightarrow> Arity \<rightarrow> AEnv"
-  assumes Aheap_eqvt[eqvt]: "\<pi> \<bullet> Aheap = Aheap"
+locale CorrectArityAnalysisHeap = CorrectArityAnalysis + ArityAnalysisHeapEqvt +
   assumes edom_Aheap: "edom (Aheap \<Gamma> e\<cdot> a) \<subseteq> domA \<Gamma>"
   assumes Aheap_subst: "x \<notin> domA \<Gamma> \<Longrightarrow> y \<notin> domA \<Gamma> \<Longrightarrow> Aheap \<Gamma>[x::h=y] e[x ::=y]  = Aheap \<Gamma> e"
 
-locale CorrectArityAnalysisLet = CorrectArityAnalysisAheap +
+locale CorrectArityAnalysisLet = CorrectArityAnalysisHeap +
   assumes Aexp_Let: "ABinds \<Gamma>\<cdot>(Aheap \<Gamma> e\<cdot>a) \<squnion> Aexp e\<cdot>a \<sqsubseteq> Aheap \<Gamma> e\<cdot>a \<squnion> Aexp (Let \<Gamma> e)\<cdot>a"
 
 locale CorrectArityAnalysisLetNoCard = CorrectArityAnalysisLet +
   assumes Aheap_heap3: "x \<in> thunks \<Gamma> \<Longrightarrow> (Aheap \<Gamma> e\<cdot>a) x = up\<cdot>0"
-
-context EdomArityAnalysis
-begin
-  lemma fup_Aexp_lookup_fresh: "atom v \<sharp> e \<Longrightarrow> (fup\<cdot>(Aexp e)\<cdot>a) v = \<bottom>"
-    by (cases a) auto
-  
-  lemma edom_AnalBinds: "edom (ABinds \<Gamma>\<cdot>ae) \<subseteq> fv \<Gamma>"
-    by (induction \<Gamma> rule: ABinds.induct)
-       (auto simp del: fun_meet_simp dest: set_mp[OF fup_Aexp_edom] dest: set_mp[OF fv_delete_subset])
-end 
 
 context SubstArityAnalysis
 begin
