Launchbury/CardinalityAnalysisSpec.thy
@@ -1,44 +1,47 @@
-theory CardinalityAnalysis
-imports ArityAnalysisSpec "Cardinality-Domain" SestoftConf ConstOn
+theory CardinalityAnalysisSpec
+imports ArityAnalysisSpec CardinalityAnalysisSig ConstOn
 begin
 
-locale CardinalityHeap = CorrectArityAnalysisLet +
-  fixes cHeap :: "heap \<Rightarrow> exp \<Rightarrow> Arity \<rightarrow> (var \<Rightarrow> two)"
+locale CardinalityPrognosisEdom = CardinalityPrognosis +
+  assumes edom_prognosis:
+    "edom (prognosis ae a (\<Gamma>, e, S)) \<subseteq> fv \<Gamma> \<union> fv e \<union> fv S"
 
-(*   assumes cHeap: "\<pi> \<bullet> cHeap = cHeap" *)
-  assumes Aheap_heap3: "x \<in> thunks \<Gamma> \<Longrightarrow> many \<sqsubseteq> (cHeap \<Gamma> e\<cdot>a) x \<Longrightarrow> (Aheap \<Gamma> e\<cdot>a) x = up\<cdot>0"
-  assumes edom_cHeap: "edom (cHeap \<Delta> e\<cdot>a) = edom (Aheap \<Delta> e\<cdot>a)"
-
-locale CardinalityPrognosis = 
-  fixes prognosis :: "AEnv \<Rightarrow> Arity \<Rightarrow> conf \<Rightarrow> (var \<Rightarrow> two)"
-
-locale CardinalityPrognosisCorrect = CardinalityPrognosis +
+locale CardinalityPrognosisShape = CardinalityPrognosis +
   assumes prognosis_env_cong: "ae f|` domA \<Gamma> = ae' f|` domA \<Gamma> \<Longrightarrow> prognosis ae u (\<Gamma>, e, S) = prognosis ae' u (\<Gamma>, e, S)"
   assumes prognosis_reorder: "map_of \<Gamma> = map_of \<Delta>  \<Longrightarrow>  prognosis ae u (\<Gamma>, e, S) = prognosis ae u (\<Delta>, e, S)"
   assumes prognosis_delete: "prognosis ae u (delete x \<Gamma>, e, S) \<sqsubseteq> prognosis ae u (\<Gamma>, e, S)"
   assumes prognosis_ap: "const_on (prognosis ae a (\<Gamma>, e, S)) (ap S) many"
   assumes prognosis_upd: "prognosis ae u (\<Gamma>, e, S) \<sqsubseteq> prognosis ae u (\<Gamma>, e, Upd x # S)"
+  assumes prognosis_not_called: "ae x = \<bottom> \<Longrightarrow> prognosis ae a (\<Gamma>, e, S) \<sqsubseteq> prognosis ae a (delete x \<Gamma>, e, S)"
+  assumes prognosis_called: "once \<sqsubseteq> prognosis ae a (\<Gamma>, Var x, S) x"
 
-
+locale CardinalityPrognosisApp = CardinalityPrognosis +
   assumes prognosis_App: "prognosis ae (inc\<cdot>a) (\<Gamma>, e, Arg x # S) \<sqsubseteq> prognosis ae a (\<Gamma>, App e x, S)"
+
+locale CardinalityPrognosisLam = CardinalityPrognosis +
   assumes prognosis_subst_Lam: "prognosis ae (pred\<cdot>a) (\<Gamma>, e[y::=x], S) \<sqsubseteq> prognosis ae a (\<Gamma>, Lam [y]. e, Arg x # S)"
+
+locale CardinalityPrognosisVar = CardinalityPrognosis +
   assumes prognosis_Var_lam: "map_of \<Gamma> x = Some e \<Longrightarrow> ae x = up\<cdot>u \<Longrightarrow> isLam e \<Longrightarrow> prognosis ae u (\<Gamma>, e, S) \<sqsubseteq> record_call x \<cdot> (prognosis ae a (\<Gamma>, Var x, S))"
   assumes prognosis_Var_thunk: "map_of \<Gamma> x = Some e \<Longrightarrow> ae x = up\<cdot>u \<Longrightarrow> \<not> isLam e \<Longrightarrow> prognosis ae u (delete x \<Gamma>, e, Upd x # S) \<sqsubseteq> record_call x \<cdot> (prognosis ae a (\<Gamma>, Var x, S))"
   assumes prognosis_Var2: "isLam e \<Longrightarrow> x \<notin> domA \<Gamma> \<Longrightarrow> prognosis ae 0 ((x, e) # \<Gamma>, e, S) \<sqsubseteq> prognosis ae 0 (\<Gamma>, e, Upd x # S)"
 
-  assumes prognosis_not_called: "ae x = \<bottom> \<Longrightarrow> prognosis ae a (\<Gamma>, e, S) \<sqsubseteq> prognosis ae a (delete x \<Gamma>, e, S)"
-
-  assumes prognosis_called: "once \<sqsubseteq> prognosis ae a (\<Gamma>, Var x, S) x"
-
-
-
-locale CardinalityPrognosisCorrectLet = CardinalityPrognosisCorrect + CardinalityHeap +
+locale CardinalityPrognosisLet = CardinalityPrognosis + CardinalityHeap + ArityAnalysisHeap +
   assumes prognosis_Let:
   "atom ` domA \<Delta> \<sharp>* \<Gamma> \<Longrightarrow> atom ` domA \<Delta> \<sharp>* S \<Longrightarrow> edom ae \<subseteq> domA \<Gamma> \<union> upds S \<Longrightarrow> prognosis (Aheap \<Delta> e\<cdot>a \<squnion> ae) a (\<Delta> @ \<Gamma>, e, S) \<sqsubseteq> cHeap \<Delta> e\<cdot>a \<squnion> prognosis ae a (\<Gamma>, Terms.Let \<Delta> e, S)"
 
-locale CardinalityPrognosisEdom = CardinalityPrognosis + CorrectArityAnalysisAheap +
-  assumes edom_prognosis:
-    "edom (prognosis ae a (\<Gamma>, e, S)) \<subseteq> fv \<Gamma> \<union> fv e \<union> fv S"
+locale CardinalityHeapCorrect = CardinalityHeap + ArityAnalysisHeap +
+  assumes Aheap_heap3: "x \<in> thunks \<Gamma> \<Longrightarrow> many \<sqsubseteq> (cHeap \<Gamma> e\<cdot>a) x \<Longrightarrow> (Aheap \<Gamma> e\<cdot>a) x = up\<cdot>0"
+  assumes edom_cHeap: "edom (cHeap \<Delta> e\<cdot>a) = edom (Aheap \<Delta> e\<cdot>a)"
 
+locale CardinalityPrognosisCorrect =
+  CardinalityPrognosisEdom +
+  CardinalityPrognosisShape +
+  CardinalityPrognosisApp +
+  CardinalityPrognosisLam + 
+  CardinalityPrognosisVar +
+  CardinalityPrognosisLet +
+  CardinalityHeapCorrect +
+  CorrectArityAnalysisLet
 
 end
