Launchbury/CoCallImplFTree.thy
@@ -1,0 +1,19 @@
+theory CoCallImplFTree
+imports FTreeAnalysisSpec CoCallAritySig "CoCallGraph-FTree"
+begin
+
+context CoCallArity
+begin
+  definition Fexp :: "exp \<Rightarrow> Arity \<rightarrow> var ftree"
+    where "Fexp e = (\<Lambda> a. ccFTree (edom (Aexp e \<cdot>a)) (ccExp e\<cdot>a))"
+  
+  lemma Fexp_simp: "Fexp e\<cdot>a = ccFTree (edom (Aexp e \<cdot>a)) (ccExp e\<cdot>a)"
+    unfolding Fexp_def by simp
+
+  sublocale FTreeAnalysis Fexp.
+end
+
+
+
+end
+
