Launchbury/FTreeImplCardinality.thy
@@ -1,0 +1,29 @@
+theory FTreeImplCardinality
+imports FTreeAnalysisSpec CardinalityAnalysisSpec CallFutureCardinality
+begin
+
+hide_const Multiset.single
+
+context FTreeAnalysis
+begin
+
+fun unstack :: "stack \<Rightarrow> exp \<Rightarrow> exp" where
+  "unstack [] e = e"
+| "unstack (Upd x # S) e = unstack S e"
+| "unstack (Arg x # S) e = unstack S (App e x)"
+| "unstack (Dummy x # S) e = unstack S e"
+
+fun Fstack :: "stack \<Rightarrow> var ftree"
+  where "Fstack [] = \<bottom>"
+  | "Fstack (Upd x # S) = Fstack S"
+  | "Fstack (Arg x # S) = many_calls x \<otimes>\<otimes> Fstack S"
+  | "Fstack (Dummy x # S) = Fstack S"
+
+lemma carrier_Fstack[simp]: "carrier (Fstack S) = ap S"
+  by (induction S rule: Fstack.induct) (auto simp add: empty_is_bottom[symmetric])
+
+fun prognosis :: "AEnv \<Rightarrow> Arity \<Rightarrow> conf \<Rightarrow> var \<Rightarrow> two"
+   where "prognosis ae a (\<Gamma>, e, S) = pathsCard (paths (substitute (FBinds \<Gamma>\<cdot>ae) (thunks \<Gamma>) (Fexp e\<cdot>a \<otimes>\<otimes> Fstack S)))"
+end
+
+end
