ROOT
@@ -35,16 +35,14 @@ session Arity (AFP) in "Launchbury" = "HOLCF-Nominal2" +
   theories
     "ArityAnalysisImpl"
     "TrivialArityAnal"
-    "ArityEtaExpand"
-    "CardinalityEtaExpand"
+    "ArityEtaExpandCorrect"
+    "CardinalityEtaExpandCorrect"
     "EtaExpansionSestoft"
     "DeadCodeRemovalCorrect"
     "DeadCodeRemoval2Correct"
     "DeadCodeRemoval2CorrectSestoft"
     "RedsImprovesArityAnalysis"
     "NoCardinalityAnalysis"
-    "FTreeCardinality"
-    "CoCallImplCorrect"
     "CallArityCorrectEnd2End"
 
 session Nominal2013_1 in "Nominal2-Isabelle2013-1/Nominal" = HOL +
